{
 "cells": [
  {
   "cell_type": "markdown",
   "metadata": {},
   "source": [
    "## Problems and applications"
   ]
  },
  {
   "cell_type": "markdown",
   "metadata": {},
   "source": [
    "1. Using the neoclassical theory of distribution (of income),\n",
    "\n",
    "* The labor force increases. Given that $MPL$ is decreasing in $L$ and $MPL = \\frac{W}{P}$, this corresponds to a fall in the real wage. Since $F(K,L)$ is increasing in $K,L$, and increase in $L$ increases the real rental rate of capital.\n",
    "\n",
    "* The capital stock falls. Then $MPK \\uparrow \\implies \\frac{R}{P} \\uparrow$. Further, $F(K,L) \\downarrow \\implies MPL \\downarrow \\implies \\frac{W}{P}$.\n",
    "\n",
    "* Under Cobb-douglas, $Y = A K^{\\alpha} L^{1-\\alpha}$. $MPL$ and $MPK$ both increasing in $A$. So $A \\uparrow \\implies \\frac{W}{P}, \\frac{R}{P}$.\n",
    "\n",
    "2. Consider the Cobb-douglas function $Y = A K^{.5} L^{.5}$, $\\overline{K} = 100, \\overline{L} = 100$.\n",
    "\n",
    "* $\\overline{Y} = F(\\overline{K},\\overline{L}) = (100)^{\\frac{1}{2}} * (100)^{\\frac{1}{2}} = 10*10 = 100$ units of output.\n",
    "\n",
    "* $MPL = (1-\\alpha)\\frac{Y}{L} = (.5)\\frac{100}{100} = .5$\n",
    "    \n",
    "    $MPK = (\\alpha)\\frac{Y}{K} = (.5)\\frac{100}{100} = .5$\n",
    "\n",
    "* Labor income = $L * MPL = (1-\\alpha)*Y = (.5)(100) = 50$.\n",
    "\n",
    "    Then, the share of total output that labor receives is $\\frac{50}{100} = .5$.\n",
    "\n",
    "* Suppose that labor falls to $L' = 50$. Then, $Y' = F(\\overline{K},L') = (100)^{\\frac{1}{2}} * (50)^{\\frac{1}{2}} = 50 \\sqrt{2}$.\n",
    "\n",
    "* $MPL = (1-\\alpha)\\frac{Y}{L} = (.5)\\frac{50 \\sqrt{2}}{50} = (\\frac{1}{2}) \\sqrt{2} \\approx .71$\n",
    "    \n",
    "    $MPK = (\\alpha)\\frac{Y}{K} = (.5)\\frac{50 \\sqrt{2}}{100} = (\\frac{1}{2}) \\frac{\\sqrt{2}}{2} \\approx .35$\n",
    "\n",
    "* $L * MPL = (1-\\alpha)*Y = (.5)(50 \\sqrt{2}) = \\approx 35.36$\n",
    "\n",
    "    Then, the share of total output that labor receives is $\\frac{\\frac{1}{2} 50 \\sqrt{2}}{50 \\sqrt{2}} = .5$.\n",
    "    "
   ]
  },
  {
   "cell_type": "markdown",
   "metadata": {},
   "source": [
    "4. When $\\alpha = .3$, then $\\overline{Y} = A \\overline{K}^{.3} \\overline{L}^{.7}$.\n",
    "\n",
    "* $\\frac{MPK * K}{Y} = \\frac{\\alpha * Y}{Y} = \\alpha$\n",
    "    \n",
    "    $\\frac{MPL * L}{Y} = \\frac{(1-\\alpha) * Y}{Y} = 1-\\alpha$\n",
    "\n",
    "    So, capital receives $.3$ or $30\\%$ of total income and labor receives $70\\%$.\n",
    "\n",
    "* Suppose labor increases by $10\\%$. Then we may write $L' = (1.1)\\overline{L}$. Then, the new level of output can be written as\n",
    "\n",
    "\\begin{gather*}\n",
    "Y' = F(\\overline{K}, L') = A \\overline{K}^{.3} ((1.1)\\overline{L})^{.7} = A \\overline{K}^{.3} \\overline{L}^{.7} * (1.1)^{.7} \\\\\n",
    "= \\overline{Y} * (1.069) \\\\\n",
    "\\end{gather*}\n",
    "\n",
    "So, we can write the percentage change in output due to the $10\\%$ increase in labor as\n",
    "\n",
    "\\begin{gather*}\n",
    "\\frac{Y' - \\overline{Y}}{\\overline{Y}} = \\frac{(1.069)*\\overline{Y} - \\overline{Y}}{\\overline{Y}} = \\frac{(1.069-1)*\\overline{Y}}{\\overline{Y}} = .069 = 6.9\\%. \\\\\n",
    "\\end{gather*} \n",
    "\n",
    "Similarly, for the change in the wage rate,\n",
    "\n",
    "\\begin{gather*}\n",
    "\\overline{MPL} = (1-\\alpha)\\frac{\\overline{Y}}{\\overline{L}}, MPL' = (1-\\alpha)\\frac{Y'}{L'} \\\\\n",
    "\\frac{MPL' - \\overline{MPL}}{\\overline{MPL}} = \\frac{(1.069)(.7)\\frac{\\overline{Y}}{\\overline{L}} - (.7)\\frac{\\overline{Y}}{\\overline{L}}}{(.7)\\frac{\\overline{Y}}{\\overline{L}}} = \\frac{\\frac{1.069}{L'} - \\frac{1}{\\overline{L}} }{\\frac{1}{\\overline{L}}} = \\frac{1.069}{(1.1)\\overline{L}} \\bigg( \\frac{\\overline{L}}{1} \\bigg) - 1 = .9718 - 1 = -.0282 =  -2.82\\%. \\\\\n",
    "\\end{gather*} \n",
    "\n",
    "And the change in the rental price of capital,\n",
    "\n",
    "\\begin{gather*}\n",
    "\\overline{MPK} = \\alpha\\frac{\\overline{Y}}{\\overline{K}}, MPK' = \\alpha\\frac{Y'}{K'} \\\\\n",
    "\\frac{MPK' - \\overline{MPK}}{\\overline{MPK}} = \\frac{(1.069)(.3)\\frac{\\overline{Y}}{\\overline{K}} - (.3)\\frac{\\overline{Y}}{\\overline{K}}}{(.3)\\frac{\\overline{Y}}{\\overline{K}}} = \\frac{(1.069-1)}{1} = .069 = 6.9\\%. \\\\\n",
    "\\end{gather*} \n",
    "\n",
    "* Replicate the steps taken in the derivations above for an increase in capital of $10\\%$.\n",
    "\n",
    "* Suppose $\\overline{A} \\uparrow$ by $10\\%$. Then $A' = (1.1)\\overline{A}$.\n",
    "\n",
    "\\begin{gather*}\n",
    "Y' = (1.1)\\overline{A} \\overline{K}^{.3} \\overline{L}^{.7} = (1.1) \\overline{Y}\\\\\n",
    "\\end{gather*}\n",
    "\n",
    "We can write the percentage change in output due to the $10\\%$ increase in labor as\n",
    "\n",
    "\\begin{gather*}\n",
    "\\frac{Y' - \\overline{Y}}{\\overline{Y}} = \\frac{(1.1)*\\overline{Y} - \\overline{Y}}{\\overline{Y}} = \\frac{(1.1-1)*\\overline{Y}}{\\overline{Y}} = .1 = 10\\%. \\\\\n",
    "\\end{gather*} \n",
    "\n",
    "For the wage rate,\n",
    "\n",
    "\\begin{gather*}\n",
    "\\overline{MPL} = (.7)\\frac{\\overline{Y}}{\\overline{L}}, MPL' = (.7)(1.1)\\frac{\\overline{Y}}{L'} \\\\\n",
    "\\frac{MPL' - \\overline{MPL}}{\\overline{MPL}} = \\frac{(1.1)(.7)\\frac{\\overline{Y}}{\\overline{L}} - (.7)\\frac{\\overline{Y}}{\\overline{L}}}{(.7)\\frac{\\overline{Y}}{\\overline{L}}} = \\frac{1.1 - 1}{1} = .1 = 10\\%.\\\\\n",
    "\\end{gather*} \n",
    "\n",
    "The same holds for $\\% \\Delta MPK = 10\\%$.\n",
    "\n"
   ]
  },
  {
   "cell_type": "markdown",
   "metadata": {},
   "source": [
    "5. From the neoclassical theory $MPL = \\frac{W}{P}$. From the assumptions of a Cobb-douglas production function $MPL = (1-\\alpha)\\frac{Y}{L}$.\n",
    "\n",
    "    Thus, if labor productivity is measured by $\\frac{Y}{L}$, it is reasonable that the wage rate tracks labor productivity.\n",
    "\n",
    "    $MPL = \\frac{W}{P}$ holds for the general specification of $F(K,L)$. With a different production function, such as increasing or decreasing returns to scale, this feature could still hold without the latter result which comes from the Cobb-douglas specification.\n",
    "\n",
    "6. According to the neoclassical theory of distribution,\n",
    "\n",
    "* $W_f , W_b \\equiv$ nominal wages $\\rightarrow$ dollars per hour\n",
    "    $P_f, P_b \\equiv$ prices $\\rightarrow$ dollars per haircut/unit of food\n",
    "    $A_f, A_b \\equiv$ marginal productivity $\\rightarrow$ output per additional barber/farmer\n",
    "\n",
    "* $A_f = \\frac{W_f}{P_f}$, so $A_f \\uparrow \\implies \\frac{W_f}{P_f} \\uparrow$. The real wage is measured in units of food per hour.\n",
    "\n",
    "* $A_b = \\frac{W_b}{P_b}$; if $A_b$ is unchanged, $\\frac{W_b}{P_b}$ is unchanged. The real wage is measured in number of haircuts per hour.\n",
    "\n",
    "* This suggests that $W_f = W_b$ in the long run. In this way, there is only one \"type\" of worker. \n",
    "\n",
    "* If $W_f = W_b$, $\\frac{W_b}{P_b} = \\frac{W_f}{P_b}$. If $P_f \\neq P_b$ and $\\frac{W_f}{P_f} \\uparrow$, then compare $\\frac{W_f}{P_f}$ and $\\frac{W_f}{P_b}$. It must be that $P_f < P_b$. Thus, $1 < \\frac{P_b}{P_f} \\implies$ the price of haircuts is higher than the price of food.\n",
    "\n",
    "* The marginal productivity of farmers increased. So, if I am a farmer, I receive the real wage of units of food per hour. From part e., $\\frac{W_f}{P_b}$, we can express the real wage of units of food per hour for barbers as well. The farmer receives more units of food per hour.\n",
    "\n",
    "    Similarly, $\\frac{W_b}{P_f} > \\frac{W_b}{P_b}$ since $P_f < P_b$ and $W_b = W_f$. Thus, the farmer benefits more from the higher technological progress since they have the same basket of consumption and farmers earn higher real wages.\n",
    "\n"
   ]
  },
  {
   "cell_type": "markdown",
   "metadata": {},
   "source": [
    "7. Consider the production function $Y = K^{\\frac{1}{3}} L^{\\frac{1}{3}} H^{\\frac{1}{3}}$.\n",
    "\n",
    "* For the marginal product of labor,\n",
    "\\begin{gather*}\n",
    "\\frac{\\partial Y}{\\partial L} = \\frac{1}{3} K^{\\frac{1}{3}} L^{\\frac{-2}{3}} H^{\\frac{1}{3}} = \\frac{1}{3} K^{\\frac{1}{3}} L^{\\frac{1}{3}} L^{\\frac{-3}{3}} H^{\\frac{1}{3}} = \\frac{1}{3} Y L^{-1}\\\\\n",
    "\\end{gather*}\n",
    "\n",
    "note, $H \\uparrow \\implies MPL \\uparrow$.\n",
    "\n",
    "* For the marginal product of human capital, \n",
    "\n",
    "\\begin{gather*}\n",
    "\\frac{\\partial Y}{\\partial L} =  K^{\\frac{1}{3}} L^{\\frac{1}{3}} \\frac{1}{3} H^{\\frac{-2}{3}}  = \\frac{1}{3} Y H^{-1}\\\\\n",
    "\\end{gather*}\n",
    "\n",
    "note, $H \\uparrow \\implies H^{-1} \\downarrow \\implies MPH \\downarrow$.\n",
    "\n",
    "* Labor income = $MPL * L = \\frac{1}{3} Y$. Human capital income = $MPH * H = \\frac{1}{3} Y$. So each receives $\\frac{1}{3}$ of the share of output.\n",
    "\n",
    "    Firms can be thought of as renting both the labor and human capital of workers. These are inputs of the production process they don't own. They do own capital though. So, from the accounting profit equation, labor income and human capital income show up in the \"economic profit\" component.\n",
    "\n",
    "* We can write unskilled wage as $W_u = MPL$ and skilled wages as $W_s = MPL + MPH$. Then,\n",
    "\n",
    "\\begin{gather*}\n",
    "\\frac{W_s}{W_u} = \\frac{MPL + MPH}{MPL} = 1 + \\frac{MPH}{MPL} = 1 + \\frac{\\frac{1}{3} Y H^{-1}}{\\frac{1}{3} Y L^{-1}} = 1 + \\frac{L}{H}\n",
    "\\end{gather*}\n",
    "\n",
    "as $H \\uparrow$, there are diminishing marginal returns to skilled labor. So, $W_s \\downarrow$ with $H \\uparrow$, meaning $\\frac{W_s}{W_u} \\downarrow$ as well.\n",
    "\n",
    "8. $T \\uparrow$ by \\$100 billion. Suppose $MPC = .6$. Then $C = C(Y-T) = .6(Y-T)$. Recall that national saving can be written in two ways:\n",
    "\n",
    "\\begin{gather*}\n",
    "S = Y - C - G \\\\\n",
    "S = (Y - T - C) + (T - G)\n",
    "\\end{gather*}\n",
    "\n",
    "* Public saving $\\equiv T - G$, so $T \\uparrow \\implies (T-G) \\uparrow$ by same amount \\$100 billion.\n",
    "\n",
    "* Private saving $\\equiv Y - T - C = Y - T - C(Y-T) = Y - T - .6(Y - T)$. \n",
    "\n",
    "    So, disposable income $(Y-T)$ falls by more than consumption $C(Y-T)$ does. Then private saving falls. $(Y-T)$ falls by \\$100 billion, $C(Y-T)$ falls by (.6) * \\$100 billion = \\$60 billion. So private saving falls by \\$40 billion.\n",
    "\n",
    "* $S = Y - C - G = Y - .6(Y-T) - G$. Since $C(Y-T)$ falls by \\$60 billion, S increases by \\$60 billion since the term $C(Y-T)$ is negative. So national saving increases by \\$60 billion.\n",
    "\n",
    "* Since $S=I$, then investment increases by the same amount, \\$60 billion. What facilitates this change in equilibrium is the interest rate.\n",
    "\n",
    "9. $Y - C(Y-T) - G = I(r)$. If $C \\uparrow$, then L.H.S. $\\downarrow \\implies$ R.H.S $\\downarrow$. This occurs when the interest rate increases."
   ]
  },
  {
   "cell_type": "markdown",
   "metadata": {},
   "source": [
    "10. Given the expressions and values describing the economy, we can solve for the following:\n",
    "\n",
    "* Public saving $= T - G = 2000 - 2500 = -500$\n",
    "    \n",
    "    Private saving = $Y - T - C = 8000 - 2000 - (1000 + \\frac{2}{3}(8000 - 2000)) = 6000 - (1000 + 4000) = 1000 $\n",
    "\n",
    "    National saving = $Y - C - G = 8000 - (1000 + \\frac{2}{3}(6000)) - 2500 = 8000-5000-2500 = 500$\n",
    "\n",
    "* $S=I$ in equilibrium. Then, the equilibrium interest rate is given by $500 = 1200 - 100r \\implies r = 7$.\n",
    "\n",
    "* Suppose $G \\downarrow by 500$. So, $G' = 2000$.\n",
    "\n",
    "    Public saving $= T - G' = 2000 - 2000 = 0$\n",
    "\n",
    "    Private saving $=Y-T-C = 1000$, since nothing changed in this expression.\n",
    "\n",
    "    National saving $= 8000 - 7000 = 1000$\n",
    "\n",
    "* The new equlibrium interest rate is the one that solves $S = I \\implies 1000 = 1200 - 100r \\implies r = 2$."
   ]
  },
  {
   "cell_type": "markdown",
   "metadata": {},
   "source": [
    "11. Recall the equilibrium condition\n",
    "\n",
    "\\begin{gather*}\n",
    "S = I \\\\\n",
    "Y - C - G = I \\\\\n",
    "Y - C(Y-T) - G = I\n",
    "\\end{gather*}\n",
    "\n",
    "So, if the MPC is equal to 1, then the balanced budget changes to taxes and government spending completely offset each other.\n",
    "\n",
    "Since the MPC is generally strictly less than 1, then the increase in government spending has a larger effect on national saving thant he increase on taxes, which effect disposable income.\n",
    "\n",
    "In this case, the LHS is smaller. So the RHS needs to be smaller, by adjustment of the interest rate. The interest rate rises then, so that the level of investment is smaller."
   ]
  },
  {
   "cell_type": "markdown",
   "metadata": {},
   "source": []
  },
  {
   "cell_type": "markdown",
   "metadata": {},
   "source": []
  },
  {
   "cell_type": "code",
   "execution_count": null,
   "metadata": {},
   "outputs": [],
   "source": []
  }
 ],
 "metadata": {
  "language_info": {
   "name": "python"
  },
  "orig_nbformat": 4
 },
 "nbformat": 4,
 "nbformat_minor": 2
}
